use genAsync on twoPhaseCommit

messageInvariantPrototypes/twoPhaseCommit/automate/distributedSystem.dfy
@@ -1,3 +1,4 @@
+/// This file is auto-generated
 include "../hosts.dfy"
 
 module Network {
@@ -5,99 +6,104 @@ module Network {
 
   datatype Variables = Variables(sentMsgs:set<Message>)
 
-  ghost predicate Init(v: Variables)
-  {
+  ghost predicate Init(v: Variables) {
     && v.sentMsgs == {}
   }
 
   ghost predicate Next(v: Variables, v': Variables, msgOps: MessageOps)
   {
-    // Only allow receipt of a message if we've seen it has been sent.
     && (msgOps.recv.Some? ==> msgOps.recv.value in v.sentMsgs)
-    // Record the sent message, if there was one.
     && v'.sentMsgs ==
       v.sentMsgs + if msgOps.send.None? then {} else { msgOps.send.value }
   }
-}
+}  // end module Network
 
 module DistributedSystem {
-  import opened UtilitiesLibrary
   import opened Types
-  import Network
+  import opened UtilitiesLibrary
+  import opened Network
   import CoordinatorHost
   import ParticipantHost
 
-  datatype Constants = Constants(
-    coordinator: seq<CoordinatorHost.Constants>,
-    participants: seq<ParticipantHost.Constants>)
-  {
-    ghost predicate WF() {
-      && CoordinatorHost.GroupWFConstants(coordinator, |participants|)
-      && ParticipantHost.GroupWFConstants(participants)
+  datatype Constants = Constants(coordinator: seq<CoordinatorHost.Constants>, participants: seq<ParticipantHost.Constants>) {
+    ghost predicate WF()
+      decreases this
+    {
+      CoordinatorHost.GroupWFConstants(coordinator, |participants|) &&
+      ParticipantHost.GroupWFConstants(participants)
     }
 
-    ghost predicate ValidParticipantId(id: HostId) {
+    ghost predicate ValidParticipantId(id: HostId)
+      decreases this, id
+    {
       id < |participants|
     }
 
-    ghost function GetCoordinator() : CoordinatorHost.Constants 
+    ghost function GetCoordinator(): CoordinatorHost.Constants
       requires WF()
+      decreases this
     {
       coordinator[0]
     }
   }
+  // end datatype Constants
 
-  datatype Hosts = Hosts(
-    coordinator: seq<CoordinatorHost.Variables>,
-    participants: seq<ParticipantHost.Variables>
-  ) {
-    ghost predicate WF(c: Constants) {
-      && c.WF()
-      && CoordinatorHost.GroupWF(c.coordinator, coordinator, |c.participants|)
-      && ParticipantHost.GroupWF(c.participants, participants)
+  datatype Hosts = Hosts(coordinator: seq<CoordinatorHost.Variables>, participants: seq<ParticipantHost.Variables>) {
+    ghost predicate WF(c: Constants)
+      decreases this, c
+    {
+      c.WF() &&
+      CoordinatorHost.GroupWF(c.coordinator, coordinator, |c.participants|) &&
+      ParticipantHost.GroupWF(c.participants, participants)
     }
 
-    ghost function GetCoordinator(c: Constants) : CoordinatorHost.Variables 
+    ghost function GetCoordinator(c: Constants): CoordinatorHost.Variables
       requires WF(c)
+      decreases this, c
     {
       coordinator[0]
     }
   }
+  // end datatype Hosts
 
   datatype Variables = Variables(
     history: seq<Hosts>,
-    network: Network.Variables)
-  {
+    network: Network.Variables
+  ) {
+  
     ghost predicate ValidHistoryIdx(i: int) {
       0 <= i < |history|
     }
-    
+  
     ghost predicate ValidHistoryIdxStrict(i: int) {
       0 <= i < |history|-1
     }
-
+  
     ghost predicate WF(c: Constants) {
       && c.WF()
       && 0 < |history|
       && (forall i | ValidHistoryIdx(i) :: history[i].WF(c))
     }
-
+  
+    ghost function Last() : (h: Hosts)
+      requires 0 < |history|
+      ensures h == history[|history|-1]
+      ensures h == History(|history|-1)
+   {
+      UtilitiesLibrary.Last(history)
+    }
+  
     ghost function History(i: int) : (h: Hosts)
       requires ValidHistoryIdx(i)
       ensures h == history[i]
     {
       history[i]
     }
+  }  // end datatype Variables
 
-    ghost function Last() : (h: Hosts) 
-      requires 0 < |history|
-      ensures h == history[|history|-1]
-    {
-      UtilitiesLibrary.Last(history)
-    }
-  } // end datatype Variables
 
   ghost predicate InitHosts(c: Constants, h: Hosts)
+    requires h.WF(c)
   {
     && CoordinatorHost.GroupInit(c.coordinator, h.coordinator)
     && ParticipantHost.GroupInit(c.participants, h.participants)
@@ -106,40 +112,42 @@ module DistributedSystem {
   ghost predicate Init(c: Constants, v: Variables)
   {
     && v.WF(c)
-    && |v.history| == 1
+   && |v.history| == 1
     && InitHosts(c, v.History(0))
     && Network.Init(v.network)
   }
 
-  ghost predicate CoordinatorAction(c: Constants, h: Hosts, h': Hosts, msgOps: MessageOps)
-    requires h.WF(c) && h'.WF(c)
-  {
-    && CoordinatorHost.Next(c.coordinator[0], h.coordinator[0], h'.coordinator[0], msgOps)
-    // all other hosts UNCHANGED
-    && h'.participants == h.participants
-  }
-
-  ghost predicate ParticipantAction(c: Constants, h: Hosts, h': Hosts, hostid: HostId, msgOps: MessageOps)
-    requires h.WF(c) && h'.WF(c)
-  {
-    && c.ValidParticipantId(hostid)
-    && ParticipantHost.Next(c.participants[hostid], h.participants[hostid], h'.participants[hostid], msgOps)
-    // all other hosts UNCHANGED
-    && h'.coordinator == h.coordinator
-    && (forall other:nat | c.ValidParticipantId(other) && other != hostid :: h'.participants[other] == h.participants[other])
-  }
-
-  datatype Step =
-    | CoordinatorStep(msgOps: MessageOps)
-    | ParticipantStep(actorIdx: nat, msgOps: MessageOps)
+  datatype Step = 
+    | CoordinatorHostStep(actor: nat, msgOps: MessageOps)
+    | ParticipantHostStep(actor: nat, msgOps: MessageOps)
 
   ghost predicate NextStep(c: Constants, h: Hosts, h': Hosts, n: Network.Variables, n': Network.Variables, step: Step)
     requires h.WF(c) && h'.WF(c)
   {
     && Network.Next(n, n', step.msgOps)
     && match step
-      case CoordinatorStep(msgOps) => CoordinatorAction(c, h, h', msgOps)
-      case ParticipantStep(actor, msgOps) => ParticipantAction(c, h, h', actor, msgOps)
+      case CoordinatorHostStep(actor, msgOps) => NextCoordinatorHostStep(c, h, h', actor, msgOps)
+      case ParticipantHostStep(actor, msgOps) => NextParticipantHostStep(c, h, h', actor, msgOps)
+  }
+
+  ghost predicate NextCoordinatorHostStep(c: Constants, h: Hosts, h': Hosts, actor: nat, msgOps: MessageOps)
+    requires h.WF(c) && h'.WF(c)
+  {
+    && 0 <= actor < |h.coordinator|
+    && CoordinatorHost.Next(c.coordinator[actor], h.coordinator[actor], h'.coordinator[actor], msgOps)
+    // all other hosts UNCHANGED
+    && (forall other| 0 <= other < |h.coordinator| && other != actor :: h'.coordinator[other] == h.coordinator[other])
+    && h'.participants == h.participants
+  }
+
+  ghost predicate NextParticipantHostStep(c: Constants, h: Hosts, h': Hosts, actor: nat, msgOps: MessageOps)
+    requires h.WF(c) && h'.WF(c)
+  {
+    && 0 <= actor < |h.participants|
+    && ParticipantHost.Next(c.participants[actor], h.participants[actor], h'.participants[actor], msgOps)
+    // all other hosts UNCHANGED
+    && h'.coordinator == h.coordinator
+    && (forall other| 0 <= other < |h.participants| && other != actor :: h'.participants[other] == h.participants[other])
   }
 
   ghost predicate Next(c: Constants, v: Variables, v': Variables)
@@ -160,7 +168,8 @@ module DistributedSystem {
     InitHosts(c, v.History(0))
   }
 
-  ghost predicate ValidVariables(c: Constants, v: Variables) 
+  // Bundle of Variable properties
+  ghost predicate ValidVariables(c: Constants, v: Variables)
     requires v.WF(c)
   {
     && ValidHistory(c, v)
@@ -172,7 +181,6 @@ module DistributedSystem {
   {
     reveal_ValidHistory();
   }
-
 
   lemma InvNextValidVariables(c: Constants, v: Variables, v': Variables)
     requires v.WF(c)
@@ -195,6 +203,5 @@ module DistributedSystem {
     assert 0 < |v.history|;
     assert 1 < |v'.history|;
   }
-} // end module Distributed System
 
-
+} // end module DistributedSystem
